Tictactoe.lean
@@ -3,4 +3,3 @@ import Tictactoe.WinningLines
 import Tictactoe.Strategy
 import Tictactoe.Proofs.Safety
 import Tictactoe.Game
-import Tictactoe.Main
